Coq/src/SimRelStep.v
@@ -43,6 +43,7 @@ Section SimRelStep.
   Variable TC : trav_config.
   Variable TC' : trav_config.
   Variable X : eventid -> Prop.
+  Variable T : thread_id -> Prop.
 
   Notation "'SE' S" := S.(ES.acts_set) (at level 10).
   Notation "'SEinit' S" := S.(ES.acts_init_set) (at level 10).
@@ -158,7 +159,7 @@ Section SimRelStep.
 
   Lemma simrel_cert_cont_pc S thread 
         (NINITT : thread <> tid_init)
-        (SRC : simrel prog S G sc TC X)
+        (SRC : simrel_consistent prog S G sc TC X T)
         (TC_STEP : isim_trav_step G sc thread TC TC') :
     exists k (state : Language.state (thread_lts thread)),
       ⟪ THK : thread = ES.cont_thread S k ⟫ /\
@@ -198,7 +199,7 @@ Section SimRelStep.
   
   Lemma simrel_cert_graph_start thread S 
         (NINITT : thread <> tid_init)
-        (SRC : simrel prog S G sc TC X) 
+        (SRC : simrel_consistent prog S G sc TC X T) 
         (TC_STEP : isim_trav_step G sc thread TC TC') : 
     exists k st st',
       ⟪ kTID : thread = ktid S k ⟫ /\
@@ -258,12 +259,12 @@ Section SimRelStep.
 
   Lemma simrel_cert_start k S 
         (st st' : thread_st (ktid S k))
-        (SRC : simrel prog S G sc TC X) 
+        (SRC : simrel_consistent prog S G sc TC X T) 
         (TC_ISTEP : isim_trav_step G sc (ktid S k) TC TC') 
         (XkTIDCOV : kE S k ≡₁ X ∩₁ e2a S ⋄₁ C ∩₁ (SEinit S ∪₁ STid S (ktid S k)))
         (CERTG : cert_graph G sc TC' (ktid S k) st')
         (CERT_ST : simrel_cstate S k st st') :
-    simrel_cert prog S G sc TC TC' X k st st'.
+    simrel_cert prog S G sc TC TC' X T k st st'.
   Proof. 
     assert (ES.Wf S) as WF by apply SRC.
     assert (Execution.t S X) as EXEC by apply SRC.
@@ -272,7 +273,7 @@ Section SimRelStep.
     { eapply sim_trav_step_coherence; try apply SRC.
       red. eauto. }
     assert (Wf G) as WFG by apply SRC.
-    assert (simrel_ prog S G sc TC X) as SR_.
+    assert (simrel prog S G sc TC X T) as SR_.
     { apply SRC. }
 
     pose proof TC_ISTEP as TT.
@@ -282,10 +283,13 @@ Section SimRelStep.
       as [lprog|] eqn:TTN; desf.
 
     constructor; auto.
+    { red; splits; [constructor|]; try apply SRC.
+      ins. eapply SRC. apply Tt. }
     (* ex_ktid_cov : X ∩₁ STid ktid ∩₁ e2a ⋄₁ C ⊆₁ kE *)
-    { generalize XkTIDCOV. basic_solver 10. }
+    { generalize XkTIDCOV. basic_solver 20. }
     (* cov_in_ex : e2a ⋄₁ C ∩₁ kE ⊆₁ X *)
     { rewrite XkTIDCOV. basic_solver. }
+    { admit. }
     (* kE_lab : eq_dom (kE \₁ SEinit) Slab (certG.(lab) ∘ e2a) *)
     { intros x [kEx nINITx].
       erewrite ex_cov_iss_lab; try apply SRC.
@@ -462,15 +466,15 @@ Section SimRelStep.
     assert ((e2a S □₁ X) x) as UU.
     { eapply ex_cov_iss.
       { apply SRC. }
-      basic_solver. }
+      red. basic_solver. }
     red in UU. desf.
     eexists. splits; eauto.
     right. by rewrite e2a_tid.
-  Qed.
+  Admitted.
 
   Lemma ew_ex_iss_cert_ex_iss k S 
         (st : thread_st (ktid S k))
-        (SRCC : simrel_cert prog S G sc TC TC' X k st st) :  
+        (SRCC : simrel_cert prog S G sc TC TC' X T k st st) :  
     dom_rel (Sew S ⨾ ⦗X ∩₁ e2a S ⋄₁ I⦘) ≡₁ 
     dom_rel (Sew S ⨾ ⦗certX S k ∩₁ e2a S ⋄₁ I⦘).
   Proof. 
@@ -485,13 +489,13 @@ Section SimRelStep.
 
   Lemma cert_ex_rf_compl k S 
         (st : thread_st (ktid S k))
-        (SRCC : simrel_cert prog S G sc TC TC' X k st st) : 
+        (SRCC : simrel_cert prog S G sc TC TC' X T k st st) : 
     certX S k ∩₁ SR S ⊆₁ codom_rel (⦗certX S k⦘ ⨾ Srf S).
   Proof. 
     assert (ES.Wf S) as WFS by apply SRCC.      
     assert (Execution.t S X) as EXEC by apply SRCC.
     assert (es_consistent S) as CONS by apply SRCC.
-    assert (simrel_ prog S G sc TC X) as SR_ by apply SRCC.
+    assert (simrel prog S G sc TC X (T \₁ eq (ktid S k))) as SR_ by apply SRCC.
     edestruct cstate_cont as [st_ [stEQ KK]]; 
       [apply SRCC|].
     red in stEQ, KK. subst st_.
@@ -543,13 +547,13 @@ Section SimRelStep.
 
   Lemma simrel_cert_vis k S
         (st : thread_st (ktid S k))
-        (SRCC : simrel_cert prog S G sc TC TC' X k st st) :
+        (SRCC : simrel_cert prog S G sc TC TC' X T k st st) :
     certX S k ⊆₁ vis S.
   Proof. 
     assert (ES.Wf S) as WFS by apply SRCC.      
     assert (Execution.t S X) as EXEC by apply SRCC.
     assert (es_consistent S) as CONS by apply SRCC.
-    assert (simrel_ prog S G sc TC X) as SR_ by apply SRCC.
+    assert (simrel prog S G sc TC X (T \₁ eq (ktid S k))) as SR_ by apply SRCC.
     edestruct cstate_cont as [st_ [stEQ KK]]; 
       [apply SRCC|].
     red in stEQ, KK. subst st_.
@@ -595,14 +599,14 @@ Section SimRelStep.
 
   Lemma simrel_cert_end k S 
         (st : thread_st (ktid S k))
-        (SRCC : simrel_cert prog S G sc TC TC' X k st st) :
-    simrel prog S G sc TC' (certX S k).
+        (SRCC : simrel_cert prog S G sc TC TC' X T k st st) :
+    simrel_consistent prog S G sc TC' (certX S k) T.
   Proof. 
     assert (ES.Wf S) as WFS.
     { apply SRCC. }
     assert (Execution.t S X) as EXEC.
     { apply SRCC. }
-    assert (simrel_ prog S G sc TC X) as SR_.
+    assert (simrel prog S G sc TC X (T \₁ eq (ktid S k))) as SR_.
     { apply SRCC. }
     assert (simrel_e2a S G sc) as SRE2A.
     { apply SRCC. }
@@ -712,7 +716,9 @@ Section SimRelStep.
       done. }
     (* ex_cov_iss : e2a □₁ certX ≡₁ C' ∪₁ dom_rel (Gsb^? ⨾ ⦗ I' ⦘) *)
     { rewrite cert_ex_certD; eauto. 
-      rewrite cert_dom_cov_sb_iss; eauto. }
+      rewrite cert_dom_cov_sb_iss; eauto. 
+      by unfold CsbI. }
+    { admit. }
     (* ex_cov_iss_lab : eq_dom (certX ∩₁ e2a ⋄₁ (C' ∪₁ I')) Slab (Glab ∘ e2a) *)
     { eapply cert_ex_cov_iss_lab; apply SRCC. }
     (* rmw_cov_in_ex : Grmw ⨾ ⦗ C' ⦘ ⊆ e2a □ Srmw ⨾ ⦗ certX ⦘ *)
@@ -766,7 +772,7 @@ Section SimRelStep.
         basic_solver. }
       rewrite id_inter, <- seqA.
       rewrite collect_rel_seqi.
-      rewrite jf_in_cert_rf; eauto.
+      rewrite jf_kE_in_cert_rf; eauto.
       rewrite collect_rel_eqv. 
       rewrite collect_map_in_set.
       rewrite set_interC.
@@ -795,11 +801,11 @@ Section SimRelStep.
     intros x HH.
     eapply rel_ew_cert_ex; eauto.
     generalize HH. basic_solver 10.
-  Qed.
+  Admitted.
 
   Lemma simrel_step_helper k S
         (st st''' : thread_st (ktid S k))
-        (SRC : simrel prog S G sc TC X)
+        (SRC : simrel_consistent prog S G sc TC X T)
         (TC_ISTEP : isim_trav_step G sc (ktid S k) TC TC')
         (XkTIDCOV : kE S k ≡₁ X ∩₁ e2a S ⋄₁ C ∩₁ (SEinit S ∪₁ STid S (ktid S k)))
         (CERTG : cert_graph G sc TC' (ktid S k) st''')
@@ -808,7 +814,7 @@ Section SimRelStep.
     (fun st' => exists k' S',
       ⟪ kTID : ktid S' k' = ktid S k ⟫ /\
       ⟪ STEPS : (step Weakestmo)＊ S S' ⟫ /\
-      ⟪ SRCC  : simrel_cert prog S' G sc TC TC' X k' st' st''' ⟫) st'''.
+      ⟪ SRCC  : simrel_cert prog S' G sc TC TC' X T k' st' st''' ⟫) st'''.
   Proof.
     eapply clos_refl_trans_ind_step_left.
     { exists k, S. splits; auto.
@@ -835,11 +841,11 @@ Section SimRelStep.
   Qed.
   
   Lemma simrel_step S 
-        (SRC : simrel prog S G sc TC X) 
+        (SRC : simrel_consistent prog S G sc TC X T) 
         (TRAV_STEP : sim_trav_step G sc TC TC') :
     exists X' S', 
       ⟪ STEPS : (step Weakestmo)＊ S S' ⟫ /\      
-      ⟪ SRC' : simrel prog S' G sc TC' X' ⟫.
+      ⟪ SRC' : simrel_consistent prog S' G sc TC' X' T⟫.
   Proof. 
     unfold sim_trav_step in TRAV_STEP. desc.
     edestruct simrel_cert_graph_start
